theories/typing.v
@@ -1,136 +1,157 @@
-Require Import imports join.
+Require Import imports par geq conv syntax.
 
-Definition context := list tm.
+Module Type typing_sig
+  (Import lattice : Lattice)
+  (Import syntax : syntax_sig lattice)
+  (Import par : par_sig lattice syntax)
+  (Import ieq : geq_sig lattice syntax)
+  (Import conv : conv_sig lattice syntax par ieq).
 
-Inductive lookup : nat -> context -> tm -> Prop :=
-  | here : forall {A Γ}, lookup 0 (A :: Γ) (A ⟨shift⟩)
-  | there : forall {n A Γ B},
-      lookup n Γ A -> lookup (S n) (B :: Γ) (A ⟨shift⟩).
+Definition context := list (T * tm).
+
+Inductive lookup : nat -> context -> T -> tm -> Prop :=
+  | here ℓ A Γ : lookup 0 ((ℓ, A) :: Γ) ℓ (A ⟨shift⟩)
+  | there n A Γ ℓ B :
+      lookup n Γ ℓ A -> lookup (S n) (B :: Γ) ℓ (A ⟨shift⟩).
 
 Definition lookup_good_renaming ξ Γ Δ :=
-  forall i A, lookup i Γ A -> lookup (ξ i) Δ A⟨ξ⟩.
+  forall i ℓ A, lookup i Γ ℓ A -> lookup (ξ i) Δ ℓ A⟨ξ⟩.
 
-Derive Inversion lookup_inv with (forall i Γ A, lookup i Γ A).
+Derive Inversion lookup_inv with (forall i Γ ℓ A, lookup i Γ ℓ A).
 
-Reserved Notation "Γ ⊢ a ∈ A" (at level 70).
+Reserved Notation "Γ ⊢ a ; ℓ ∈ A" (at level 70).
 Reserved Notation "⊢ Γ" (at level 70).
 
-Inductive Wt : context -> tm -> tm -> Prop :=
-| T_Var Γ i A :
+Definition c2e : context -> econtext := map (fun '(ℓ, _) => ℓ).
+
+Inductive Wt : context -> T -> tm -> tm -> Prop :=
+| T_Var Γ ℓ0 ℓ i A :
   ⊢ Γ ->
-  lookup i Γ A ->
+  lookup i Γ ℓ0 A ->
+  ℓ0 ⊆ ℓ ->
   (* ------ *)
-  Γ ⊢ (var_tm i) ∈ A
+  Γ ⊢ (var_tm i) ; ℓ ∈ A
 
-| T_Pi Γ i A B :
-  Γ ⊢ A ∈ (tUniv i) ->
-  (A :: Γ) ⊢ B ∈ (tUniv i) ->
+| T_Pi Γ i ℓ ℓ0 A B :
+  Γ ⊢ A ; ℓ ∈ (tUniv i) ->
+  ((ℓ0, A) :: Γ) ⊢ B ; ℓ ∈ (tUniv i) ->
   (* --------------------- *)
-  Γ ⊢ (tPi A B) ∈ (tUniv i)
+  Γ ⊢ (tPi ℓ0 A B) ; ℓ ∈ (tUniv i)
 
-| T_Abs Γ A a B i :
-  Γ ⊢ (tPi A B) ∈ (tUniv i) ->
-  (A :: Γ) ⊢ a ∈ B ->
+| T_Abs Γ ℓ ℓ0 ℓ1 A a B i :
+  Γ ⊢ (tPi ℓ0 A B) ; ℓ1 ∈ (tUniv i) ->
+  ((ℓ0, A) :: Γ) ⊢ a ; ℓ ∈ B ->
   (* -------------------- *)
-  Γ ⊢ (tAbs a) ∈ (tPi A B)
+  Γ ⊢ (tAbs ℓ0 a) ; ℓ ∈ (tPi ℓ0 A B)
 
-| T_App Γ a A B b :
-  Γ ⊢ a ∈ (tPi A B) ->
-  Γ ⊢ b ∈ A ->
+| T_App Γ ℓ ℓ0 a A B b :
+  Γ ⊢ a ; ℓ ∈ (tPi ℓ0 A B) ->
+  Γ ⊢ b ; ℓ0 ∈ A ->
   (* -------------------- *)
-  Γ ⊢ (tApp a b) ∈ (B [ b.. ])
+  Γ ⊢ (tApp a ℓ0 b) ; ℓ ∈ (B [ b.. ])
 
-| T_Conv Γ a A B i :
-  Γ ⊢ a ∈ A ->
-  Γ ⊢ B ∈ (tUniv i) ->
-  A <: B ->
+| T_Conv Γ ℓ ℓ0 a A B i :
+  Γ ⊢ a ; ℓ ∈ A ->
+  Γ ⊢ B ; ℓ0 ∈ (tUniv i) ->
+  conv (c2e Γ) A B ->
   (* ----------- *)
-  Γ ⊢ a ∈ B
+  Γ ⊢ a ; ℓ ∈ B
 
-| T_Zero Γ :
+(* | T_Zero Γ : *)
+(*   ⊢ Γ -> *)
+(*   (* --------- *) *)
+(*   Γ ⊢ tZero ∈ tNat *)
+
+(* | T_Suc Γ a : *)
+(*   Γ ⊢ a ∈ tNat -> *)
+(*   ⊢ Γ -> *)
+(*   (* --------- *) *)
+(*   Γ ⊢ tSuc a ∈ tNat *)
+
+(* | T_Ind Γ a b c A i : *)
+(*   tNat :: Γ ⊢ A ∈ tUniv i -> *)
+(*   Γ ⊢ a ∈ A [tZero..] -> *)
+(*   A :: tNat :: Γ ⊢ b ∈ A[tSuc (var_tm 0) .: S >> var_tm]⟨S⟩ -> *)
+(*   Γ ⊢ c ∈ tNat -> *)
+(*   (* ------------ *) *)
+(*   Γ ⊢ tInd a b c ∈ (A [c..]) *)
+
+(* | T_Nat Γ i : *)
+(*   ⊢ Γ -> *)
+(*   (* ----------- *) *)
+(*   Γ ⊢ tNat ∈ (tUniv i) *)
+
+| T_Univ Γ ℓ i :
   ⊢ Γ ->
-  (* --------- *)
-  Γ ⊢ tZero ∈ tNat
-
-| T_Suc Γ a :
-  Γ ⊢ a ∈ tNat ->
-  ⊢ Γ ->
-  (* --------- *)
-  Γ ⊢ tSuc a ∈ tNat
-
-| T_Ind Γ a b c A i :
-  tNat :: Γ ⊢ A ∈ tUniv i ->
-  Γ ⊢ a ∈ A [tZero..] ->
-  A :: tNat :: Γ ⊢ b ∈ A[tSuc (var_tm 0) .: S >> var_tm]⟨S⟩ ->
-  Γ ⊢ c ∈ tNat ->
   (* ------------ *)
-  Γ ⊢ tInd a b c ∈ (A [c..])
+  Γ ⊢ (tUniv i) ; ℓ ∈ (tUniv (S i))
 
-| T_Nat Γ i :
-  ⊢ Γ ->
-  (* ----------- *)
-  Γ ⊢ tNat ∈ (tUniv i)
-
-| T_Univ Γ i :
+| T_Void Γ ℓ i :
   ⊢ Γ ->
   (* ------------ *)
-  Γ ⊢ (tUniv i) ∈ (tUniv (S i))
+  Γ ⊢ tVoid ; ℓ ∈ tUniv i
 
-| T_Refl Γ a A:
-  ⊢ Γ ->
-  Γ ⊢ a ∈ A ->
-  (* ------ *)
-  Γ ⊢ tRefl ∈ (tEq a a A)
+| T_Absurd Γ ℓ0 ℓ1 i a A :
+  Γ ⊢ a ; ℓ0 ∈ tVoid  ->
+  Γ ⊢ A ; ℓ1 ∈ tUniv i ->
+  (* -------------- *)
+  Γ ⊢ a ; ℓ0 ∈ A
 
-| T_Eq Γ a b A i j :
-  Γ ⊢ a ∈ A ->
-  Γ ⊢ b ∈ A ->
-  Γ ⊢ A ∈ (tUniv j) ->
-  (* ----------------------- *)
-  Γ ⊢ (tEq a b A) ∈ (tUniv i)
+(* | T_Refl Γ a A: *)
+(*   ⊢ Γ -> *)
+(*   Γ ⊢ a ∈ A -> *)
+(*   (* ------ *) *)
+(*   Γ ⊢ tRefl ∈ (tEq a a A) *)
 
-| T_J Γ t a b p A i j C : 
-  Γ ⊢ a ∈  A ->
-  Γ ⊢ b ∈ A ->
-  Γ ⊢ A ∈ (tUniv j) ->
-  Γ ⊢ p ∈ (tEq a b A) ->
-  (tEq (ren_tm shift a) (var_tm 0) (ren_tm shift A) :: A :: Γ) ⊢ C ∈ (tUniv i) ->
-  Γ ⊢ t ∈ (C [tRefl .: a ..]) ->
-  Γ ⊢ (tJ t a b p) ∈ (C [p .: b..])
+(* | T_Eq Γ a b A i j : *)
+(*   Γ ⊢ a ∈ A -> *)
+(*   Γ ⊢ b ∈ A -> *)
+(*   Γ ⊢ A ∈ (tUniv j) -> *)
+(*   (* ----------------------- *) *)
+(*   Γ ⊢ (tEq a b A) ∈ (tUniv i) *)
 
-| T_Sig Γ i A B :
-  Γ ⊢ A ∈ (tUniv i) ->
-  (A :: Γ) ⊢ B ∈ (tUniv i) ->
-  (* --------------------- *)
-  Γ ⊢ (tSig A B) ∈ (tUniv i)
+(* | T_J Γ t a b p A i j C :  *)
+(*   Γ ⊢ a ∈  A -> *)
+(*   Γ ⊢ b ∈ A -> *)
+(*   Γ ⊢ A ∈ (tUniv j) -> *)
+(*   Γ ⊢ p ∈ (tEq a b A) -> *)
+(*   (tEq (ren_tm shift a) (var_tm 0) (ren_tm shift A) :: A :: Γ) ⊢ C ∈ (tUniv i) -> *)
+(*   Γ ⊢ t ∈ (C [tRefl .: a ..]) -> *)
+(*   Γ ⊢ (tJ t a b p) ∈ (C [p .: b..]) *)
 
-| T_Pack Γ a A b B i :
-  Γ ⊢ a ∈ A ->
-  Γ ⊢ b ∈ B[a..] ->
-  Γ ⊢ tSig A B ∈ tUniv i ->
-  (* -------------------- *)
-  Γ ⊢ tPack a b ∈ tSig A B
+(* | T_Sig Γ i A B : *)
+(*   Γ ⊢ A ∈ (tUniv i) -> *)
+(*   (A :: Γ) ⊢ B ∈ (tUniv i) -> *)
+(*   (* --------------------- *) *)
+(*   Γ ⊢ (tSig A B) ∈ (tUniv i) *)
 
-| T_Let Γ a b A B C i j :
-  Γ ⊢ A ∈ tUniv j ->
-  A :: Γ ⊢ B ∈ tUniv j ->
-  Γ ⊢ a ∈ tSig A B ->
-  B :: A :: Γ ⊢ b ∈ C[(tPack (var_tm 1) (var_tm 0)) .: (shift >> shift >> var_tm)] ->
-  tSig A B :: Γ ⊢ C ∈ tUniv i ->
-  (* ----------------------- *)
-  Γ ⊢ tLet a b ∈ C[a ..]
+(* | T_Pack Γ a A b B i : *)
+(*   Γ ⊢ a ∈ A -> *)
+(*   Γ ⊢ b ∈ B[a..] -> *)
+(*   Γ ⊢ tSig A B ∈ tUniv i -> *)
+(*   (* -------------------- *) *)
+(*   Γ ⊢ tPack a b ∈ tSig A B *)
+
+(* | T_Let Γ a b A B C i j : *)
+(*   Γ ⊢ A ∈ tUniv j -> *)
+(*   A :: Γ ⊢ B ∈ tUniv j -> *)
+(*   Γ ⊢ a ∈ tSig A B -> *)
+(*   B :: A :: Γ ⊢ b ∈ C[(tPack (var_tm 1) (var_tm 0)) .: (shift >> shift >> var_tm)] -> *)
+(*   tSig A B :: Γ ⊢ C ∈ tUniv i -> *)
+(*   (* ----------------------- *) *)
+(*   Γ ⊢ tLet a b ∈ C[a ..] *)
 
 with Wff : context -> Prop :=
 | Wff_nil :
 (* ----------------- *)
   ⊢ nil
-| Wff_cons Γ A i :
+| Wff_cons Γ ℓ0 ℓ A i :
   ⊢ Γ ->
-  Γ ⊢ A ∈ tUniv i ->
+  Γ ⊢ A ; ℓ ∈ tUniv i ->
 (* ----------------- *)
-  ⊢ A :: Γ
+  ⊢ (ℓ0, A) :: Γ
 where 
-  "Γ ⊢ a ∈ A" := (Wt Γ a A) and "⊢ Γ" := (Wff Γ).
+  "Γ ⊢ a ; ℓ ∈ A" := (Wt Γ ℓ a A) and "⊢ Γ" := (Wff Γ).
 
 
 Scheme wt_ind := Induction for Wt Sort Prop
